theories/util/types.v
@@ -1,46 +1,89 @@
 From stdpp Require Import prelude.
+From iris.algebra Require Import ofe.
 
 (** * List of Types *)
 (** We avoid using [list Type] because that can cause universe inconsistency *)
 
-Inductive Types := NilTypes: Types | ConsTypes: Type → Types → Types.
-Implicit Type As Bs: Types.
+Inductive Types := tnil: Types | tcons: Type → Types → Types.
+Implicit Type As: Types.
 
-Notation "^[ ]" := (NilTypes) (at level 5, format "^[ ]").
-Infix "^::" := (ConsTypes) (at level 60, right associativity).
+Notation "^[ ]" := (tnil) (at level 5, format "^[ ]").
+Infix "^::" := (tcons) (at level 60, right associativity).
 Notation "^[ A ; .. ; B ]" := (A ^:: .. (B ^:: ^[]) ..)
   (at level 5, format "^[ A ;  .. ;  B ]").
 
+Fixpoint app_Types As Bs :=
+  match As with ^[] => Bs | A ^:: As' => A ^:: app_Types As' Bs end.
+Infix "^++" := (app_Types) (at level 60, right associativity).
+
 (** * Heterogeneous List *)
 
-Inductive hlist (F: Type → Type) : Types → Type :=
-| NilHlist: hlist F ^[]
-| ConsHlist {A As} : F A → hlist F As → hlist F (A ^:: As).
+Inductive hlist F : Types → Type :=
+| hnil: hlist F ^[]
+| hcons {A As} : F A → hlist F As → hlist F (A ^:: As).
 
-Notation "+[ ]" := (NilHlist _) (at level 1, format "+[ ]").
-Notation "+[ ]@{ F }" := (NilHlist F) (at level 1, only parsing).
-Infix "+::" := (ConsHlist _) (at level 60, right associativity).
-Infix "+::@{ F }" := (ConsHlist F)
-  (at level 60, right associativity, only parsing).
-Notation "+[ a ; .. ; z ]" := (a +:: .. (z +:: +[]) ..)
-  (at level 1, format "+[ a ;  .. ;  z ]").
-Notation "+[ a ; .. ; z ]@{ F }" := (a +:: .. (z +:: +[]@{F}) ..)
+Notation "+[ ]" := (hnil _) (at level 1, format "+[ ]").
+Notation "+[ ]@{ F }" := (hnil F) (at level 1, only parsing).
+Infix "+::" := (hcons _) (at level 60, right associativity).
+Infix "+::@{ F }" := (hcons F) (at level 60, right associativity, only parsing).
+Notation "+[ x ; .. ; z ]" := (x +:: .. (z +:: +[]) ..)
+  (at level 1, format "+[ x ;  .. ;  z ]").
+Notation "+[ x ; .. ; z ]@{ F }" := (x +:: .. (z +:: +[]@{F}) ..)
   (at level 1, only parsing).
+
+Fixpoint happ {F As Bs} (xl: hlist F As) (yl: hlist F Bs)
+  : hlist F (As ^++ Bs) :=
+  match xl with +[] => yl | x +:: xl' => x +:: happ xl' yl end.
+Infix "+++" := (happ) (at level 60, right associativity).
+
+Fixpoint hmap {F As B} (f: ∀A, F A → B) (xl: hlist F As) : list B :=
+  match xl with +[] => [] | x +:: xl' => f _ x :: hmap f xl' end.
+Infix "+<$>" := (hmap) (at level 61, left associativity).
+
+Inductive HForall {F} (Φ: ∀A, F A → Prop) : ∀{As: Types}, hlist F As → Prop :=
+| HForall_nil: HForall Φ +[]
+| HForall_cons {A As} (x: _ A) (xl: _ As) :
+    Φ _ x → HForall Φ xl → HForall Φ (x +:: xl).
+
+Inductive HForall2 {F G} (Φ: ∀A, F A → G A → Prop)
+  : ∀{As: Types}, hlist F As → hlist G As → Prop :=
+| HForall2_nil: HForall2 Φ +[] +[]
+| HForall2_cons {A As} (x: _ A) (y: _ A) (xl: _ As) (yl: _ As) :
+    Φ _ x y → HForall2 Φ xl yl → HForall2 Φ (x +:: xl) (y +:: yl).
+
+Section setoid.
+Context {F: Type → Type} `{∀A, Equiv (F A)}.
+
+Global Instance hlist_equiv {As} : Equiv (hlist F As) := HForall2 (λ _, (≡)).
+
+End setoid.
+
+Section ofe.
+Context {F: Type → ofe}.
+
+Global Instance hlist_dist {As} : Dist (hlist F As) :=
+  λ n, HForall2 (λ _, dist n).
+Global Instance hcons_ne {A As} : NonExpansive2 (@hcons F A As).
+Proof. move=> ???????. by apply HForall2_cons. Qed.
+
+End ofe.
 
 (** * List-like Product *)
 
-Inductive nil_unit := NilTt: nil_unit.
-Inductive cons_prod A B := ConsPair: A → B → cons_prod A B.
-Arguments ConsPair {_ _} _ _.
+Inductive nil_unit := nil_tt: nil_unit.
+Inductive cons_prod A B := cons_pair: A → B → cons_prod A B.
+Arguments cons_pair {_ _} _ _.
 
-Notation ":1" := (nil_unit) (at level 1).
-Infix ":*" := (cons_prod) (at level 39, right associativity).
-Notation "-[ ]" := (NilTt) (at level 1, format "-[ ]").
-Infix "-::" := (ConsPair) (at level 60, right associativity).
+Notation ":1" := (nil_unit) (at level 1) : type_scope.
+Infix ":*" := (cons_prod) (at level 60, right associativity) : type_scope.
+Notation "-[ ]" := (nil_tt) (at level 1, format "-[ ]").
+Infix "-::" := (cons_pair) (at level 60, right associativity).
 Notation "-[ a ; .. ; z ]" := (a -:: .. (z -:: -[]) ..)
   (at level 1, format "-[ a ;  .. ;  z ]").
 
-Fixpoint flist As : Type := match As with
-| ^[] => :1
-| A ^:: As => A :* flist As
-end.
+Fixpoint flist F As : Type :=
+  match As with ^[] => :1 | A ^:: As' => F A :* flist F As' end.
+Fixpoint app_flist {F As Bs} (xl: flist F As) (yl: flist F Bs)
+  : flist F (As ^++ Bs) := match As, xl with
+  | ^[], -[] => yl | A ^:: As', x -:: xl' => x -:: app_flist xl' yl end.
+Infix "-++" := (app_flist) (at level 60, right associativity).
